A rather ugly fix for #39

PermutLib.v
@@ -4,7 +4,6 @@ Require Export LibList.
 Require Export LibFset.
 Require Export LibRelation.
 
-
 Notation " Ctx *=* Ctx'" := (permut Ctx Ctx') (at level 70) : permut_scope.
 
 Lemma Permut_refl:
@@ -106,11 +105,270 @@ intros; apply Mem_split; eapply Mem_permut; eauto;
 apply Mem_here.
 Qed.
 
+Section OtherDefinition.
+
+Variable A:Type.
+
+Inductive Permutation : list A -> list A -> Prop :=
+| perm_nil: Permutation nil nil
+| perm_skip x l l' : Permutation l l' -> Permutation (x::l) (x::l')
+| perm_swap x y l : Permutation (y::x::l) (x::y::l)
+| perm_trans l l' l'' :
+  Permutation l l' -> Permutation l' l'' -> Permutation l l''.
+
+Local Hint Constructors Permutation.
+
+Theorem Permutation_refl : forall l : list A, Permutation l l.
+Proof.
+  induction l; constructor. exact IHl.
+Qed.
+
+Theorem Permutation_sym : forall l l' : list A, Permutation l l' ->
+  Permutation l' l.
+Proof.
+  intros l l' Hperm; induction Hperm; auto.
+  apply perm_trans with (l':=l'); assumption.
+Qed.
+
+Theorem Permutation_trans : forall l l' l'' : list A, Permutation l l' ->
+  Permutation l' l'' -> Permutation l l''.
+Proof.
+  exact perm_trans.
+Qed.
+
+Hint Resolve Permutation_refl perm_nil perm_skip.
+
+(* These hints do not reduce the size of the problem to solve and they
+   must be used with care to avoid combinatoric explosions *)
+
+Local Hint Resolve perm_swap perm_trans.
+Local Hint Resolve Permutation_sym Permutation_trans.
+
+(* This provides reflexivity, symmetry and transitivity and rewriting
+   on morphims to come *)
+
+Instance Permutation_Equivalence : Equivalence (Permutation) | 10 := {
+  Equivalence_Reflexive := Permutation_refl ;
+  Equivalence_Symmetric := Permutation_sym ;
+  Equivalence_Transitive := Permutation_trans }.
+
+Add Parametric Morphism (a:A) : (cons a)
+  with signature Permutation ==> Permutation
+  as Permutation_cons.
+Proof.
+  auto using perm_skip.
+Qed.
+
+
+
+Theorem Permutation_nil : forall (l : list A), Permutation nil l -> l = nil.
+Proof.
+  intros l HF.
+  remember (@nil A) as m in HF.
+  induction HF; discriminate || auto.
+Qed.
+
+Theorem Permutation_nil_cons : forall (l : list A) (x : A),
+  ~ Permutation nil (x::l).
+Proof.
+  intros l x HF.
+  apply Permutation_nil in HF; discriminate.
+Qed.
+
+Lemma Permutation_app_tail : forall (l l' tl : list A), Permutation l l' ->
+  Permutation (l++tl) (l'++tl).
+Proof.
+  intros l l' tl Hperm; induction Hperm as [|x l l'|x y l|l l' l'']; rew_app;
+    simpl; auto.
+  eapply Permutation_trans with (l':=l'++tl); trivial.
+Qed.
+
+Lemma Permutation_app_head : forall (l tl tl' : list A), Permutation tl tl' ->
+  Permutation (l++tl) (l++tl').
+Proof.
+  intros l tl tl' Hperm; induction l; [trivial |
+    repeat rewrite <- app_comm_cons; constructor; assumption].
+Qed.
+
+Theorem Permutation_app : forall (l m l' m' : list A), Permutation l l' ->
+  Permutation m m' -> Permutation (l++m) (l'++m').
+Proof.
+  intros l m l' m' Hpermll' Hpermmm'; induction Hpermll' as
+    [|x l l'|x y l|l l' l'']; repeat rewrite <- app_comm_cons; rew_app; auto.
+  apply Permutation_trans with (l' := (x :: y :: l) ++ m);
+	[rew_app | ]; auto. replace (x::y::l++m') with ((x::y::l)++m') by
+  (rew_app; auto);
+          apply Permutation_app_head; auto.
+  apply Permutation_trans with (l' := (l' ++ m')); try assumption.
+  apply Permutation_app_tail; assumption.
+Qed.
+
+Add Parametric Morphism : (@append A)
+  with signature Permutation ==> Permutation ==> Permutation
+  as Permutation_app'.
+  intros; auto using Permutation_app.
+Qed.
+
+Lemma Permutation_add_inside : forall a (l l' tl tl' : list A),
+  Permutation l l' -> Permutation tl tl' ->
+  Permutation (l ++ a :: tl) (l' ++ a :: tl').
+Proof.
+  intros; apply Permutation_app; auto.
+Qed.
+
+Theorem Permutation_app_comm : forall (l l' : list A),
+  Permutation (l ++ l') (l' ++ l).
+Proof.
+  induction l as [|x l]; simpl; intro l'.
+  rew_app; trivial.
+  induction l' as [|y l']; simpl.
+  rew_app; trivial.
+  transitivity (x :: y :: l' ++ l).
+  constructor; rew_app; apply IHl.
+  transitivity (y :: x :: l' ++ l); constructor.
+  transitivity (x :: l ++ l'); auto.
+Qed.
+
+Theorem Permutation_cons_app : forall (l l1 l2:list A) a,
+  Permutation l (l1 ++ l2) -> Permutation (a :: l) (l1 ++ a :: l2).
+Proof.
+  intros l l1; revert l.
+  induction l1.
+  simpl.
+  intros; apply perm_skip; auto.
+  simpl; intros.
+  transitivity (a0::a::l1++l2).
+  apply perm_skip; auto.
+  transitivity (a::a0::l1++l2).
+  apply perm_swap; auto.
+  rew_app; apply perm_skip; auto.
+Qed.
+Local Hint Resolve Permutation_cons_app.
+
+Theorem Permutation_in : forall (l l' : list A) (x : A), Permutation l l' ->
+  In x l -> In x l'.
+Proof.
+  intros l l' x Hperm; induction Hperm; simpl; tauto.
+Qed.
+
+Lemma Permutation_swap_middle:
+forall l1 l2 l3 l4,
+  Permutation (l1 ++ l2 ++ l3 ++ l4) (l1 ++ l3 ++ l2 ++ l4).
+intros;
+apply Permutation_app_head;
+replace (l2 ++ l3 ++ l4) with ((l2 ++ l3) ++ l4) by (rew_app; auto);
+replace (l3 ++ l2 ++ l4) with ((l3 ++ l2) ++ l4) by (rew_app; auto);
+apply Permutation_app_tail;
+apply Permutation_app_comm.
+Qed.
+
+Lemma Permutation_Mem:
+forall (l l' : list A) (x : A), Permutation l l' -> Mem x l -> Mem x l'.
+intros. induction H; auto.
+rewrite Mem_cons_eq in H0; destruct H0; subst;
+[apply Mem_here | rewrite Mem_cons_eq]; right; apply IHPermutation; auto.
+repeat rewrite Mem_cons_eq in *; destruct H0; subst.
+right; left; auto. destruct H; subst; [left | right]; auto.
+Qed.
+
+Theorem permut_equiv:
+forall l1 l2,
+  l1 *=* l2 <->
+  Permutation l1 l2.
+split; intro.
+generalize dependent l2;
+generalize dependent l1;
+apply rtclosure_ind; intros; auto;
+transitivity y; auto; inversion H; subst; apply Permutation_swap_middle.
+induction H; permut_simpl; auto; transitivity l'; auto.
+Qed.
+
+Theorem Permutation_ind_bis :
+ forall P : list A -> list A -> Prop,
+   P nil nil ->
+   (forall x l l', Permutation l l' -> P l l' -> P (x :: l) (x :: l')) ->
+   (forall x y l l', Permutation l l' -> P l l' ->
+     P (y :: x :: l) (x :: y :: l')) ->
+   (forall l l' l'', Permutation l l' -> P l l' ->
+     Permutation l' l'' -> P l' l'' -> P l l'') ->
+   forall l l', Permutation l l' -> P l l'.
+Proof.
+  intros P Hnil Hskip Hswap Htrans.
+  intros; induction H; auto.
+  apply Htrans with (x::y::l); auto.
+  apply Hswap; auto.
+  induction l; auto.
+  apply Hskip; auto.
+  apply Hskip; auto.
+  induction l; auto.
+  eauto.
+Qed.
+
+Ltac break_list l x l' H :=
+  destruct l as [|x l']; simpl in *;
+  injection H; intros; subst; clear H.
+
+Theorem Permutation_app_inv : forall (l1 l2 l3 l4:list A) a,
+  Permutation (l1++a::l2) (l3++a::l4) -> Permutation (l1++l2) (l3 ++ l4).
+Proof.
+  set (P l l' :=
+         forall a l1 l2 l3 l4, l=l1++a::l2 -> l'=l3++a::l4 ->
+           Permutation (l1++l2) (l3++l4)).
+  cut (forall l l', Permutation l l' -> P l l').
+  intros; apply (H _ _ H0 a); auto.
+  intros; apply (Permutation_ind_bis P); unfold P; clear P;
+    try clear H l l'; simpl; auto.
+(* nil *)
+  intros; destruct l1; simpl in *; discriminate.
+  (* skip *)
+  intros x l l' H IH; intros.
+  break_list l1 b l1' H0; break_list l3 c l3' H1.
+  auto.
+  apply perm_trans with (l3'++c::l4); rew_app; auto.
+  apply perm_trans with (l1'++a::l2); rew_app; auto using Permutation_cons_app.
+  rew_app; apply perm_skip.
+  apply (IH a l1' l2 l3' l4); auto.
+  (* contradict *)
+  intros x y l l' Hp IH; intros.
+  break_list l1 b l1' H; break_list l3 c l3' H0; rew_app;
+  auto.
+  break_list l3' b l3'' H; rew_app;
+  auto.
+  apply perm_trans with (c::l3''++b::l4); auto.
+  break_list l1' c l1'' H1; rew_app;
+  auto.
+  apply perm_trans with (b::l1''++c::l2); auto.
+  break_list l3' d l3'' H; break_list l1' e l1'' H1; rew_app;
+  auto.
+  apply perm_trans with (e::a::l1''++l2); auto.
+  apply perm_trans with (e::l1''++a::l2); auto.
+  apply perm_trans with (d::a::l3''++l4); auto.
+  apply perm_trans with (d::l3''++a::l4); auto.
+  apply perm_trans with (e::d::l1''++l2); auto.
+  apply perm_skip; apply perm_skip.
+  apply (IH a l1'' l2 l3'' l4); auto.
+  (*trans*)
+  intros.
+  destruct (Mem_split A l' a) as (l'1, (l'2, H6)).
+    apply Permutation_Mem with (l:=a::l1++l2).
+    subst; rewrite <- H; auto.
+    apply Mem_here.
+  apply perm_trans with (l'1++l'2).
+  rew_app in *; apply (H0 _ _ _ _ _ H3 H6).
+  rew_app in *; apply (H2 _ _ _ _ _ H6 H4).
+Qed.
+
+End OtherDefinition.
+
 Lemma permut_app_inv:
 forall A l1 l2 l3 l4 (a:A),
   l1 & a ++ l2 *=* l3 & a ++ l4 ->
   l1 ++ l2 *=* l3 ++ l4.
-Admitted. (* !!! Bug: #39 *)
+intros.
+apply permut_equiv.
+apply Permutation_app_inv with (a:=a).
+eapply permut_equiv; rew_app in *; eauto.
+Qed.
 
 Lemma permut_cons_inv:
 forall A l1 l2 (a:A),
@@ -163,20 +421,57 @@ repeat rewrite notin_union in *; destruct H0; destruct H;
 repeat split; try (rewrite from_list_nil; apply notin_empty); auto.
 Qed.
 
+Lemma Mem_dec:
+forall A (l: list A) e
+  (Dec: forall k k':A, { k = k' } + {~ k = k'}),
+  {Mem e l} + {~ Mem e l}.
+induction l; intros; [ right; rewrite Mem_nil_eq; tauto | ].
+assert (forall k k' : A, {k = k'} + {k <> k'}) as DecP by auto.
+specialize Dec with e a; destruct Dec; subst; rewrite Mem_cons_eq.
+left; left; auto.
+specialize IHl with e; apply IHl in DecP; destruct DecP; [ left | right].
+right; auto. intro nn; destruct nn; subst; [ elim n | contradiction]; auto.
+Qed.
+
+(* This is the decidability as in DecidableEquivalence class *)
+Lemma permut_Dec:
+forall A (a: list A) a'
+  (Dec: forall k k':A, {k = k'} + {~k = k'}),
+  (permut a a') \/ (~permut a a').
+induction a; intros.
+destruct a'; [left | right]; auto;
+intro; apply permut_nil_eq in H; inversion H.
+assert ({Mem a a'} + {~ Mem a a'}) as H by (apply Mem_dec; auto);
+destruct H.
+(* Mem a a' *)
+apply Mem_split in m; destruct m as (hd, (tl, m)).
+specialize IHa with (a':=hd++tl); apply IHa in Dec; destruct Dec;
+[ left | right ]; subst.
+rewrite H; permut_simpl.
+intro; elim H. apply permut_cons_inv with (a:=a); rewrite H0; permut_simpl.
+(* ~ Mem a a' *)
+right; intro;
+apply permut_split_head in H; destruct H as (hd, (tl, H)); subst;
+repeat rewrite Mem_app_or_eq in n; elim n; left; right; apply Mem_here.
+Qed.
+
 Lemma permut_dec:
 forall A (a: list A) a'
   (Dec: forall k k':A, {k = k'} + {~k = k'}),
   { permut a a' } + { ~permut a a' }.
-induction a; intros; destruct a'; [left | right | right |].
-auto.
+induction a; intros.
+destruct a'; [left | right]; auto;
 intro; apply permut_nil_eq in H; inversion H.
-intro; symmetry in H; apply permut_nil_eq in H; inversion H.
-assert (forall k k' : A, {k = k'} + {k <> k'}) as DecP by auto;
-specialize Dec with a a1; destruct Dec; subst.
-apply IHa with (a':=a') in DecP;
-destruct DecP; [left | right]; auto;
-intro; apply permut_cons_inv in H; contradiction.
-(* now, if a <> a1 there's no simple way to use IHa with just a':=a *)
+assert ({Mem a a'} + {~ Mem a a'}) as H by (apply Mem_dec; auto);
+destruct H.
+(* Mem a a' *)
+apply Mem_split in m.
+(* We'd like to use destruct m here *)
+Focus 2.
+(* ~ Mem a a' *)
+right; intro;
+apply permut_split_head in H; destruct H as (hd, (tl, H)); subst;
+repeat rewrite Mem_app_or_eq in n; elim n; left; right; apply Mem_here.
 Admitted. (* !!! Bug: #38 *)
 
 Lemma notin_Mem:
